wip on rst

NLustre/MemSemantics2.v
@@ -69,112 +69,70 @@ Module Type MEMSEMANTICS
        (Import NoD   : NODUP       Ids Op       Clks Syn         Mem IsD IsV)
        (Import WeF   : WELLFORMED  Ids Op       Clks Syn     Ord Mem IsD IsV IsF NoD).
 
-  Definition memory := memory (stream val).
+  Definition memories := stream (memory val).
 
-  Definition sfalse : cstream := fun n => false.
-
-  Definition merge_reset (rs rs': cstream) : cstream :=
-    fun n => rs n || rs' n.
-
-  Inductive mfby: cstream -> ident -> val -> stream value -> memory -> stream value -> Prop :=
+  Inductive mfby: cstream -> ident -> val -> stream value -> memories -> stream value -> Prop :=
     mfby_intro:
-      forall (r: cstream) x v0 ls M xs ms,
-        mfind_mem x M = Some ms ->
-        ms 0 = v0 ->
-        (forall n,
-            let rst_n := if r n then v0 else ms n in
-            match ls n with
-              | absent    => ms (S n) = rst_n /\ xs n = absent
-              | present v => ms (S n) = v     /\ xs n = present rst_n
+      forall (r: cstream) x v0 ls M xs,
+        mfind_mem x (M 0) = Some v0 ->
+        (forall n, match mfind_mem x (M n) with
+              | Some mv =>
+                match ls n with
+                | absent    =>
+                  mfind_mem x (M (S n)) = Some (if r (S n) then v0 else mv)
+                  /\ xs n = absent
+                | present v =>
+                  mfind_mem x (M (S n)) = Some (if r (S n) then v0 else v)
+                  /\ xs n = present mv
+                end
+              | None => False
               end) ->
         mfby r x v0 ls M xs.
 
-  (* Lemma mask'_S: *)
-  (*   forall {A} k rs (xs ys: stream A) n, *)
-  (*     mask' k rs xs ys -> *)
-  (*     (count rs n = k ->  *)
-  (*      ys (S n) = xs (S n) \/ ys (S n) = ys n. *)
-  (* Admitted. *)
-
-  (* Lemma foo: *)
-  (*   forall x v0 ls M xs k rs M', *)
-  (*     mfby x v0 ls M xs -> *)
-  (*     mmask k rs M M' -> *)
-  (*     mfby x v0 (mask absent k rs ls) M' (mask absent k rs xs). *)
-  (* Proof. *)
-  (*   intros ** Fby Mask. *)
-  (*   inversion_clear Fby as [?????? Find ? Spec]. *)
-  (*   apply Mask in Find as (ms' & ? & Mask'). *)
-  (*   (* pose proof Mask' as MaskS. *) *)
-  (*   destruct Mask' as (Hinit & Spec'). *)
-  (*   econstructor; eauto. *)
-  (*   - now rewrite Hinit. *)
-  (*   - pose proof Spec' as SpecS; *)
-  (*       intro n; specialize (Spec n); specialize (Spec' n); *)
-  (*         specialize (SpecS (S n)); simpl in *. *)
-  (*     unfold mask. *)
-  (*     destruct (EqNat.beq_nat k (count rs n)) eqn: E. *)
-  (*     + destruct (rs (S n)). *)
-  (*       *{ apply EqNat.beq_nat_true in E. *)
-  (*          destruct (EqNat.beq_nat k (S (count rs n))) eqn: E'. *)
-  (*          - apply EqNat.beq_nat_true in E'; rewrite E in E'; omega. *)
-  (*          - destruct (ls n); intuition. *)
-  (*            + admit. *)
-  (*            + now rewrite Spec'. *)
-  (*        } *)
-  (*       *{ rewrite E in SpecS. *)
-  (*          destruct (ls n); intuition. *)
-  (*          - now rewrite SpecS, Spec'. *)
-  (*          - now rewrite SpecS. *)
-  (*          - now rewrite Spec'. *)
-  (*        } *)
-  (*     + destruct (rs (S n)). *)
-  (*       * destruct (EqNat.beq_nat k (S (count rs n))) eqn: E'; intuition. *)
-  (*         admit. *)
-  (*       * rewrite E in SpecS. *)
-  (*         intuition. *)
-  (* Qed. *)
-
-  Implicit Type M : memory.
-
   Section NodeSemantics.
+
+    Definition sub_inst_n (x: ident) (M M': memories) : Prop :=
+      forall n, sub_inst x (M n) (M' n).
+
+    Definition or_str (bs1 bs2: cstream) : cstream :=
+      fun n => bs1 n || bs2 n.
 
     Variable G: global.
 
-    Inductive msem_equation: cstream -> cstream -> history -> memory -> equation -> Prop :=
+    Inductive msem_equation: cstream -> cstream -> history -> memories -> equation -> Prop :=
     | SEqDef:
-        forall bk r H M x ck xs ce,
+        forall bk rk H M x ck xs ce,
           sem_var bk H x xs ->
           sem_caexp bk H ck ce xs ->
-          msem_equation bk r H M (EqDef x ck ce)
+          msem_equation bk rk H M (EqDef x ck ce)
     | SEqApp:
-        forall bk r H M x xs ck f M' arg ls xss,
+        forall bk rk H M x xs ck f M' arg ls xss,
           Some x = hd_error xs ->
-          mfind_inst x M = Some M' ->
+          sub_inst_n x M M' ->
           sem_laexps bk H ck arg ls ->
           sem_vars bk H xs xss ->
-          msem_node r f ls M' xss ->
-          msem_equation bk r H M (EqApp xs ck f arg None)
+          msem_node f rk ls M' xss ->
+          msem_equation bk rk H M (EqApp xs ck f arg None)
     | SEqReset:
-        forall bk r H M x xs ck f M' arg y ck_r ys ls xss,
+        forall bk rk H M x xs ck f M' arg r ck_r ys ls xss,
           Some x = hd_error xs ->
-          mfind_inst x M = Some M' ->
+          sub_inst_n x M M' ->
           sem_laexps bk H ck arg ls ->
           sem_vars bk H xs xss ->
-          sem_var bk H y ys ->
-          msem_node (merge_reset r (reset_of ys)) f ls M' xss ->
-          msem_equation bk r H M (EqApp xs ck f arg (Some (y, ck_r)))
+          sem_avar bk H ck_r r ys ->
+          msem_node f (or_str rk (reset_of ys)) ls M' xss ->
+          msem_equation bk rk H M (EqApp xs ck f arg (Some (r, ck_r)))
     | SEqFby:
-        forall bk r H M x ck ls xs c0 le,
+        forall bk rk H M x ck ls xs c0 le,
           sem_laexp bk H ck le ls ->
           sem_var bk H x xs ->
-          mfby r x (sem_const c0) ls M xs ->
-          msem_equation bk r H M (EqFby x ck c0 le)
+          mfby rk x (sem_const c0) ls M xs ->
+          msem_equation bk rk H M (EqFby x ck c0 le)
 
     with msem_node:
-           cstream -> ident -> stream (list value) -> memory -> stream (list value) -> Prop :=
+           ident -> cstream -> stream (list value) -> memories -> stream (list value) -> Prop :=
          | SNode:
-             forall bk r H f xss M yss n,
+             forall bk rk H f xss M yss n,
                clock_of xss bk ->
                find_node f G = Some n ->
                sem_vars bk H (map fst n.(n_in)) xss ->
@@ -182,10 +140,10 @@ Module Type MEMSEMANTICS
                same_clock xss ->
                same_clock yss ->
                (forall n, absent_list (xss n) <-> absent_list (yss n)) ->
-               Forall (msem_equation bk r H M) n.(n_eqs) ->
-               msem_node r f xss M yss.
+               Forall (msem_equation bk rk H M) n.(n_eqs) ->
+               msem_node f rk xss M yss.
 
-    Definition msem_equations bk r H M eqs := Forall (msem_equation bk r H M) eqs.
+    Definition msem_equations bk rk H M eqs := Forall (msem_equation bk rk H M) eqs.
 
   End NodeSemantics.
 
@@ -199,45 +157,45 @@ enough: it does not support the internal fixpoint introduced by
 
     Variable G: global.
 
-    Variable P_equation: cstream -> cstream -> history -> memory -> equation -> Prop.
-    Variable P_node: cstream -> ident -> stream (list value) -> memory -> stream (list value) -> Prop.
+    Variable P_equation: cstream -> cstream -> history -> memories -> equation -> Prop.
+    Variable P_node: ident -> cstream -> stream (list value) -> memories -> stream (list value) -> Prop.
 
     Hypothesis EqDefCase:
-      forall bk r H M x ck xs ce,
+      forall bk rk H M x ck xs ce,
         sem_var bk H x xs ->
         sem_caexp bk H ck ce xs ->
-        P_equation bk r H M (EqDef x ck ce).
+        P_equation bk rk H M (EqDef x ck ce).
 
     Hypothesis EqAppCase:
-      forall bk r H M x xs ck f M' arg ls xss,
+      forall bk rk H M x xs ck f M' arg ls xss,
         Some x = hd_error xs ->
-        mfind_inst x M = Some M' ->
+        sub_inst_n x M M' ->
         sem_laexps bk H ck arg ls ->
         sem_vars bk H xs xss ->
-        msem_node G r f ls M' xss ->
-        P_node r f ls M' xss ->
-        P_equation bk r H M (EqApp xs ck f arg None).
+        msem_node G f rk ls M' xss ->
+        P_node f rk ls M' xss ->
+        P_equation bk rk H M (EqApp xs ck f arg None).
 
     Hypothesis EqResetCase:
-      forall bk r H M x xs ck f M' arg y ck_r ys ls xss,
+      forall bk rk H M x xs ck f M' arg r ck_r ys ls xss,
         Some x = hd_error xs ->
-        mfind_inst x M = Some M' ->
+        sub_inst_n x M M' ->
         sem_laexps bk H ck arg ls ->
         sem_vars bk H xs xss ->
-        sem_var bk H y ys ->
-        msem_node G (merge_reset r (reset_of ys)) f ls M' xss ->
-        P_node (merge_reset r (reset_of ys)) f ls M' xss ->
-        P_equation bk r H M (EqApp xs ck f arg (Some (y, ck_r))).
+        sem_avar bk H ck_r r ys ->
+        msem_node G f (or_str rk (reset_of ys)) ls M' xss ->
+        P_node f (or_str rk (reset_of ys)) ls M' xss ->
+        P_equation bk rk H M (EqApp xs ck f arg (Some (r, ck_r))).
 
     Hypothesis EqFbyCase:
-      forall bk r H M x ck ls xs c0 le,
+      forall bk rk H M x ck ls xs c0 le,
         sem_laexp bk H ck le ls ->
         sem_var bk H x xs ->
-        mfby r x (sem_const c0) ls M xs ->
-        P_equation bk r H M (EqFby x ck c0 le).
+        mfby rk x (sem_const c0) ls M xs ->
+        P_equation bk rk H M (EqFby x ck c0 le).
 
     Hypothesis NodeCase:
-      forall bk r H f xss M yss n,
+      forall bk rk H f xss M yss n,
         clock_of xss bk ->
         find_node f G = Some n ->
         sem_vars bk H (map fst n.(n_in)) xss ->
@@ -245,101 +203,94 @@ enough: it does not support the internal fixpoint introduced by
         same_clock xss ->
         same_clock yss ->
         (forall n, absent_list (xss n) <-> absent_list (yss n)) ->
-        Forall (msem_equation G bk r H M) n.(n_eqs) ->
-        Forall (P_equation bk r H M) n.(n_eqs) ->
-        P_node r f xss M yss.
+        Forall (msem_equation G bk rk H M) n.(n_eqs) ->
+        Forall (P_equation bk rk H M) n.(n_eqs) ->
+        P_node f rk xss M yss.
 
     Fixpoint msem_equation_mult
-             (b r: cstream) (H: history) (M: memory) (e: equation)
+             (b r: cstream) (H: history) (M: memories) (e: equation)
              (Sem: msem_equation G b r H M e) {struct Sem}
       : P_equation b r H M e
     with msem_node_mult
-           (r: cstream)
            (f: ident)
+           (r: cstream)
            (xss: stream (list value))
-           (M: memory)
+           (M: memories)
            (oss: stream (list value))
-           (Sem: msem_node G r f xss M oss) {struct Sem}
-         : P_node r f xss M oss.
+           (Sem: msem_node G f r xss M oss) {struct Sem}
+         : P_node f r xss M oss.
     Proof.
       - destruct Sem; eauto.
       - destruct Sem; eauto.
         eapply NodeCase; eauto.
-        (* clear H1 defd vout good. *)
         induction H7; auto.
     Qed.
 
-    Combined Scheme msem_equation_node_ind from msem_equation_mult, msem_node_mult.
+    Combined Scheme msem_equation_node_reset_ind from
+             msem_equation_mult, msem_node_mult.
 
   End msem_node_mult.
 
+  Definition falses: cstream := fun n => false.
+
   Definition msem_nodes (G: global) : Prop :=
-    Forall (fun no => exists xs M ys, msem_node G sfalse no.(n_name) xs M ys) G.
+    Forall (fun no => exists xs M ys, msem_node G no.(n_name) falses xs M ys) G.
 
   (** ** Properties *)
 
   (** *** Equation non-activation *)
 
-  (* Lemma subrate_property_eqn: *)
-  (*   forall G H M bk xss eqn n, *)
-  (*     clock_of xss bk -> *)
-  (*     msem_equation G bk H M eqn -> *)
-  (*     0 < length (xss n) -> *)
-  (*     absent_list (xss n) -> *)
-  (*     rhs_absent_instant (bk n) (restr H n) eqn. *)
-  (* Proof. *)
-  (*   intros * Hck Hsem Hlen Habs. *)
-  (*   assert (Hbk: bk n = false). *)
-  (*   { *)
-  (*     destruct (Bool.bool_dec (bk n) false) as [Hbk | Hbk]; eauto. *)
-  (*     exfalso. *)
-  (*     apply Bool.not_false_is_true in Hbk. *)
-  (*     eapply Hck in Hbk. *)
-  (*     eapply not_absent_present_list in Hbk; auto. *)
-  (*   } *)
-  (*   rewrite Hbk in *. *)
-  (*   destruct eqn. *)
-  (*   constructor. *)
-  (*   apply SCabs; try apply subrate_clock. *)
+  Lemma subrate_property_eqn:
+    forall G H M bk rk xss eqn n,
+      clock_of xss bk ->
+      msem_equation G bk rk H M eqn ->
+      0 < length (xss n) ->
+      absent_list (xss n) ->
+      rhs_absent_instant (bk n) (restr H n) eqn.
+  Proof.
+    intros * Hck Hsem Hlen Habs.
+    assert (Hbk: bk n = false).
+    {
+      destruct (Bool.bool_dec (bk n) false) as [Hbk | Hbk]; eauto.
+      exfalso.
+      apply Bool.not_false_is_true in Hbk.
+      eapply Hck in Hbk.
+      eapply not_absent_present_list in Hbk; auto.
+    }
+    induction Hsem as [????????? Hsem |
+                       ?????????????? Hsem |
+                       ????????????????? Hsem ? Hvar |
+                       ?????????? Hsem];
+      unfold sem_caexp, lift in Hsem; specialize (Hsem n); inv Hsem;
+        try (exfalso; rewrite Hbk in *; now eapply not_subrate_clock; eauto).
+    - eauto using rhs_absent_instant, sem_caexp_instant.
+    - econstructor.
+      + apply SLabss; eauto.
+      + match goal with H: ls n = _ |- _ => rewrite H end; apply all_absent_spec.
+    - unfold sem_avar, lift in Hvar; specialize (Hvar n); inv Hvar;
+        try (exfalso; rewrite Hbk in *; now eapply not_subrate_clock; eauto).
+      econstructor.
+      + apply SLabss; eauto.
+      + match goal with H: ls n = _ |- _ => rewrite H end; apply all_absent_spec.
+      (* + eauto using sem_avar_instant. *)
+    - eauto using rhs_absent_instant, sem_laexp_instant.
+  Qed.
 
-  (*   ; *)
-  (*     try repeat *)
-  (*         match goal with *)
-  (*         | |- rhs_absent_instant false _ (EqDef _ _ _) => *)
-  (*           constructor *)
-  (*         | |- rhs_absent_instant false _ (EqFby _ _ _ _) => *)
-  (*           constructor *)
-  (*         | |- sem_caexp_instant false _ ?ck ?ce absent => *)
-  (*           apply SCabs *)
-  (*         | |- sem_clock_instant false _ ?ck false => *)
-  (*           apply subrate_clock *)
-  (*         | |- sem_laexp_instant false _ ?ck ?le absent => *)
-  (*           apply SLabs *)
-  (*         | |- sem_laexps_instant false _ ?ck ?les _ => *)
-  (*           apply SLabss; eauto *)
-  (*         end. *)
-  (*   clear Hsem Habs. *)
-  (*   apply AEqApp with (vs:=map (fun _ =>absent) l). *)
-  (*   apply SLabss; auto. apply subrate_clock. *)
-  (*   induction l; [constructor|]. *)
-  (*   apply Forall_cons; auto. *)
-  (* Qed. *)
-
-  (* Lemma subrate_property_eqns: *)
-  (*   forall G H M bk xss eqns n, *)
-  (*     clock_of xss bk -> *)
-  (*     msem_equations G bk H M eqns -> *)
-  (*     0 < length (xss n) -> *)
-  (*     absent_list (xss n) -> *)
-  (*     Forall (rhs_absent_instant (bk n) (restr H n)) eqns. *)
-  (* Proof. *)
-  (*   intros * Hck Hsem Habs. *)
-  (*   induction eqns as [|eqn eqns]; auto. *)
-  (*   inversion_clear Hsem. *)
-  (*   constructor. *)
-  (*   eapply subrate_property_eqn; eauto. *)
-  (*   eapply IHeqns; eauto. *)
-  (* Qed. *)
+  Lemma subrate_property_eqns:
+    forall G H M bk rk xss eqns n,
+      clock_of xss bk ->
+      msem_equations G bk rk H M eqns ->
+      0 < length (xss n) ->
+      absent_list (xss n) ->
+      Forall (rhs_absent_instant (bk n) (restr H n)) eqns.
+  Proof.
+    intros * Hck Hsem Habs.
+    induction eqns as [|eqn eqns]; auto.
+    inversion_clear Hsem.
+    constructor.
+    eapply subrate_property_eqn; eauto.
+    eapply IHeqns; eauto.
+  Qed.
 
   (** *** Environment cons-ing lemmas *)
 
@@ -351,20 +302,20 @@ enough: it does not support the internal fixpoint introduced by
    TODO: try this when the other elements are stabilised. *)
 
   Lemma msem_node_cons:
-    forall n G r f xs M ys,
+    forall n G f rk xs M ys,
       Ordered_nodes (n :: G) ->
-      msem_node (n :: G) r f xs M ys ->
+      msem_node (n :: G) f rk xs M ys ->
       n.(n_name) <> f ->
-      msem_node G r f xs M ys.
+      msem_node G f rk xs M ys.
   Proof.
     Hint Constructors msem_equation.
     intros ** Hord Hsem Hnf.
     revert Hnf.
     induction Hsem as [| | | |????????? Hf ?????? IH]
         using msem_node_mult
-      with (P_equation := fun bk r H M eq =>
+      with (P_equation := fun bk rk H M eq =>
                             ~Is_node_in_eq n.(n_name) eq ->
-                            msem_equation G bk r H M eq); eauto.
+                            msem_equation G bk rk H M eq); eauto.
     - intro Hnin.
       econstructor; eauto.
       apply IHHsem. intro Hnf; apply Hnin; rewrite Hnf. constructor.
@@ -382,11 +333,11 @@ enough: it does not support the internal fixpoint introduced by
   Qed.
 
   Lemma msem_node_cons2:
-    forall n G r f xs M ys,
+    forall n G f rk xs M ys,
       Ordered_nodes G ->
-      msem_node G r f xs M ys ->
+      msem_node G f rk xs M ys ->
       Forall (fun n' => n_name n <> n_name n') G ->
-      msem_node (n :: G) r f xs M ys.
+      msem_node (n :: G) f rk xs M ys.
   Proof.
     Hint Constructors msem_equation.
     intros ** Hord Hsem Hnin.
@@ -394,9 +345,9 @@ enough: it does not support the internal fixpoint introduced by
     revert Hnin'.
     induction Hsem as [| | | |??????? n' ? Hfind ????? Heqs IH]
         using msem_node_mult
-      with (P_equation := fun bk r H M eq =>
+      with (P_equation := fun bk rk H M eq =>
                             ~Is_node_in_eq n.(n_name) eq ->
-                            msem_equation (n :: G) bk r H M eq); eauto.
+                            msem_equation (n :: G) bk rk H M eq); eauto.
     intro HH; clear HH.
     assert (n.(n_name) <> f) as Hnf.
     { intro Hnf.
@@ -443,11 +394,11 @@ enough: it does not support the internal fixpoint introduced by
   Qed.
 
   Lemma msem_equation_cons2:
-    forall G bk r H M eqs n,
+    forall G bk rk H M eqs n,
       Ordered_nodes (n :: G) ->
-      Forall (msem_equation G bk r H M) eqs ->
+      Forall (msem_equation G bk rk H M) eqs ->
       ~Is_node_in n.(n_name) eqs ->
-      Forall (msem_equation (n :: G) bk r H M) eqs.
+      Forall (msem_equation (n :: G) bk rk H M) eqs.
   Proof.
     Hint Constructors msem_equation.
     intros ** Hord Hsem Hnini.
@@ -466,10 +417,10 @@ enough: it does not support the internal fixpoint introduced by
     forall G f,
       msem_nodes G ->
       find_node f G <> None ->
-      exists xs M ys,
-        msem_node G sfalse f xs M ys.
+      exists xs M ys rk,
+        msem_node G f rk xs M ys.
   Proof.
-    intros G f Hnds Hfind.
+    intros ** Hnds Hfind.
     apply find_node_Exists in Hfind.
     apply Exists_exists in Hfind.
     destruct Hfind as [nd [Hin Hf]].
@@ -477,19 +428,19 @@ enough: it does not support the internal fixpoint introduced by
     rewrite Forall_forall in Hnds.
     apply Hnds in Hin.
     destruct Hin as [xs [M [ys Hmsem]]].
-    exists xs; exists M; exists ys.
+    exists xs, M, ys, falses.
     rewrite Hf in *.
     exact Hmsem.
   Qed.
 
   (* TODO: Tidy this up... *)
   Lemma Forall_msem_equation_global_tl:
-    forall n G bk r H M eqs,
+    forall n G bk rk H M eqs,
       Ordered_nodes (n :: G) ->
       (forall f, Is_node_in f eqs -> find_node f G <> None) ->
       ~ Is_node_in n.(n_name) eqs ->
-      Forall (msem_equation (n :: G) bk r H M) eqs ->
-      Forall (msem_equation G bk r H M) eqs.
+      Forall (msem_equation (n :: G) bk rk H M) eqs ->
+      Forall (msem_equation G bk rk H M) eqs.
   Proof.
     intros ??????? Hord.
     induction eqs as [|eq eqs IH]; trivial; [].
@@ -512,31 +463,41 @@ enough: it does not support the internal fixpoint introduced by
 
   (** *** Memory management *)
 
-  Lemma mfby_madd_mem:
-    forall r x v0 ls M xs y ms,
+  Definition add_mems (y: ident) (ms: stream val) (M: memories): memories :=
+    fun n => madd_mem y (ms n) (M n).
+
+  Lemma mfby_add_mems:
+    forall rk x v0 ls M xs y ms,
       x <> y ->
-      mfby r x v0 ls M xs ->
-      mfby r x v0 ls (madd_mem y ms M) xs.
+      mfby rk x v0 ls M xs ->
+      mfby rk x v0 ls (add_mems y ms M) xs.
   Proof.
-    inversion 2; econstructor; eauto.
-    rewrite mfind_mem_gso; auto.
+    unfold add_mems.
+    intros ** Fby; inversion_clear Fby as [??????? Spec].
+    constructor.
+    - rewrite mfind_mem_gso; auto.
+    - intro n; rewrite 2 mfind_mem_gso; auto.
+      exact (Spec n).
   Qed.
 
-  Lemma mfby_madd_obj:
-    forall r x v0 ls M xs y M',
-      mfby r x v0 ls M xs ->
-      mfby r x v0 ls (madd_obj y M' M) xs.
+  Definition add_objs (y: ident) (M' M: memories): memories :=
+    fun n => madd_obj y (M' n) (M n).
+
+  Lemma mfby_add_objs:
+    forall rk x v0 ls M xs y M',
+      mfby rk x v0 ls M xs ->
+      mfby rk x v0 ls (add_objs y M' M) xs.
   Proof.
     inversion 1; econstructor; eauto.
   Qed.
 
-  Hint Resolve mfby_madd_mem mfby_madd_obj.
+  Hint Resolve mfby_add_mems mfby_add_objs.
 
   Lemma msem_equation_madd_mem:
-    forall G bk r H M x ms eqs,
+    forall G bk rk H M x ms eqs,
       ~Is_defined_in_eqs x eqs ->
-      Forall (msem_equation G bk r H M) eqs ->
-      Forall (msem_equation G bk r H (madd_mem x ms M)) eqs.
+      Forall (msem_equation G bk rk H M) eqs ->
+      Forall (msem_equation G bk rk H (add_mems x ms M)) eqs.
   Proof.
     Hint Constructors msem_equation.
     intros ** Hnd Hsem.
@@ -552,10 +513,10 @@ enough: it does not support the internal fixpoint introduced by
   Qed.
 
   Lemma msem_equation_madd_obj:
-    forall G bk r H M M' x eqs,
+    forall G bk rk H M M' x eqs,
       ~Is_defined_in_eqs x eqs ->
-      Forall (msem_equation G bk r H M) eqs ->
-      Forall (msem_equation G bk r H (madd_obj x M' M)) eqs.
+      Forall (msem_equation G bk rk H M) eqs ->
+      Forall (msem_equation G bk rk H (add_objs x M' M)) eqs.
   Proof.
     Hint Constructors msem_equation.
     intros * Hnd Hsem.
@@ -568,10 +529,11 @@ enough: it does not support the internal fixpoint introduced by
     destruct Hsem as [|???? x' ??????? Hsome
                          |???? x' ?????????? Hsome|];
       eauto;
-      assert (mfind_inst x' (madd_obj x M' M) = Some M'0)
+      assert (sub_inst_n x' (add_objs x M' M) M'0)
         by (apply not_Is_defined_in_eq_EqApp in Hnd;
-            rewrite mfind_inst_gso; auto;
-            intro; subst x; destruct xs; inv Hsome; apply Hnd; now constructor);
+            unfold sub_inst_n, sub_inst, add_objs in *; intro;
+            rewrite mfind_inst_gso; auto; intro; subst x; destruct xs;
+            inv Hsome; apply Hnd; now constructor);
       eauto.
   Qed.
 
@@ -617,27 +579,29 @@ dataflow memory for which the non-standard semantics holds true.
    *)
 
   Lemma sem_msem_eq:
-    forall G bk H eqs M eq mems argIn,
+    forall G bk rk H eqs M eq mems argIn,
+      rk = falses ->
       (forall f xs ys,
           sem_node G f xs ys ->
-          exists M, msem_node G sfalse f xs M ys) ->
-      (forall r f xs ys,
+          exists M, msem_node G f rk xs M ys) ->
+      (forall f r xs ys,
           sem_reset G f r xs ys ->
-          exists M, msem_node G r f xs M ys) ->
+          exists M, msem_node G f (or_str rk r) xs M ys) ->
       sem_equation G bk H eq ->
       Is_well_sch mems argIn (eq :: eqs) ->
-      Forall (msem_equation G bk sfalse H M) eqs ->
-      exists M', Forall (msem_equation G bk sfalse H M') (eq :: eqs).
+      Forall (msem_equation G bk rk H M) eqs ->
+      exists M', Forall (msem_equation G bk rk H M') (eq :: eqs).
   Proof.
     intros ** IH IH' Heq Hwsch Hmeqs.
-    inversion Heq as [|? ? ? ? ? ? ? ? Hls Hxs Hsem
-                         |? ? ? ? ? ? ? ? ? ? ? Hls Hxs Hy Hsem
-                         |? ? ? ? ? ? ? ? Hle Hvar];
+    subst rk.
+    inversion Heq as [|???????? Hls Hxs Hsem
+                         |??????????? Hls Hxs Hy Hsem
+                         |???????? Hle Hvar];
       match goal with H:_=eq |- _ => rewrite <-H in * end.
     - exists M.
       repeat (econstructor; eauto).
     - apply IH in Hsem as [M' Hmsem].
-      exists (madd_obj (hd Ids.default x) M' M).
+      exists (add_objs (hd Ids.default x) M' M).
 
       assert (exists i, Some i = hd_error x) as [i Hsome].
       {
@@ -674,7 +638,7 @@ dataflow memory for which the non-standard semantics holds true.
 
       constructor.
       + econstructor; eauto.
-        now apply mfind_inst_gss.
+        unfold sub_inst, add_objs; intro; now apply mfind_inst_gss.
       + inversion_clear Hwsch.
         assert (Is_defined_in_eq i (EqApp x ck f arg None)).
         {
@@ -685,7 +649,7 @@ dataflow memory for which the non-standard semantics holds true.
 
     - pose proof Hsem as Hsem'.
       apply IH' in Hsem as [M' Hmsem].
-      exists (madd_obj (hd Ids.default x) M' M).
+      exists (add_objs (hd Ids.default x) M' M).
 
       assert (exists i, Some i = hd_error x) as [i Hsome].
       {
@@ -697,11 +661,10 @@ dataflow memory for which the non-standard semantics holds true.
           assert (exists n, length (map fst n.(n_out)) = length (xs 0)
                        /\ 0 < length n.(n_out)) as (n & ? & ?).
           {
-            inversion_clear Hmsem as [? ? ? ? ? Hmsem'].
-            (* destruct (Hmsem' 0) as (? & ? & Hmsem); inv Hmsem. *)
+            inversion_clear Hmsem as [??????????? Hout].
             exists n; split; auto.
-            - unfold sem_vars, lift in H9; specialize (H9 0).
-              apply Forall2_length in H9; now rewrite H9.
+            - unfold sem_vars, lift in Hout; specialize (Hout 0).
+              apply Forall2_length in Hout; now rewrite Hout.
             - exact n.(n_outgt0).
           }
 
@@ -725,7 +688,7 @@ dataflow memory for which the non-standard semantics holds true.
 
       constructor.
       + econstructor; eauto.
-        now apply mfind_inst_gss.
+        unfold sub_inst, add_objs; intro. now apply mfind_inst_gss.
       + inversion_clear Hwsch.
         assert (Is_defined_in_eq i (EqApp x ck f arg (Some (y, ck_r)))).
         {
@@ -734,13 +697,16 @@ dataflow memory for which the non-standard semantics holds true.
         }
         apply msem_equation_madd_obj; auto.
 
-    - exists (madd_mem x (hold (sem_const c0) ls) M).
+    - exists (add_mems x (hold (sem_const c0) ls) M).
+      subst.
       constructor.
-      + do 2 (econstructor; eauto).
+      + unfold add_mems.
+        do 2 (econstructor; eauto).
         * now apply mfind_mem_gss.
-        * reflexivity.
-        * rewrite H1; unfold fby; simpl.
-          intro n; destruct (ls n); auto.
+        (* * reflexivity. *)
+        * unfold fby; simpl.
+          intro n; destruct (ls n); auto;
+            repeat rewrite mfind_mem_gss; auto.
       + inversion_clear Hwsch.
         apply msem_equation_madd_mem; eauto.
   Qed.
@@ -748,19 +714,20 @@ dataflow memory for which the non-standard semantics holds true.
   (* XXX: for this lemma, and the ones before/after it, factorize 'G',
 'bk' and possibly other variables in a Section *)
   Corollary sem_msem_eqs:
-    forall G bk H eqs mems argIn,
+    forall G bk rk H eqs mems argIn,
+      rk = falses ->
       (forall f xs ys,
           sem_node G f xs ys ->
-          exists M, msem_node G sfalse f xs M ys) ->
-      (forall r f xs ys,
+          exists M, msem_node G f rk xs M ys) ->
+      (forall f r xs ys,
           sem_reset G f r xs ys ->
-          exists M, msem_node G r f xs M ys) ->
+          exists M, msem_node G f (or_str rk r) xs M ys) ->
       Is_well_sch mems argIn eqs ->
       Forall (sem_equation G bk H) eqs ->
-      exists M', Forall (msem_equation G bk sfalse H M') eqs.
+      exists M', Forall (msem_equation G bk rk H M') eqs.
   Proof.
     intros ** IH Hwsch Heqs.
-    induction eqs as [|eq eqs IHeqs]; [exists (empty_memory _); now constructor|].
+    induction eqs as [|eq eqs IHeqs]; [exists (fun n => empty_memory _); now constructor|].
     apply Forall_cons2 in Heqs as [Heq Heqs].
     eapply IHeqs with (1:=Is_well_sch_cons _ _ _ _ Hwsch)
       in Heqs
@@ -768,11 +735,82 @@ dataflow memory for which the non-standard semantics holds true.
     eapply sem_msem_eq; eauto.
   Qed.
 
+  Lemma instant_inv_msem_equation:
+    forall G bk rk H M eq,
+      ((exists x ck ce xs,
+           eq = EqDef x ck ce
+           /\ (forall k,
+                 sem_var_instant (restr H k) x (xs k)
+                 /\ sem_caexp_instant (bk k) (restr H k) ck ce (xs k)))
+       \/
+       (exists xs ck f arg ls x M' xss,
+           eq = EqApp xs ck f arg None
+           /\ Some x = hd_error xs
+           /\ msem_node G f rk ls M' xss
+           /\ (forall k,
+                 sub_inst x (M k) (M' k)
+                 /\ sem_laexps_instant (bk k) (restr H k) ck arg (ls k)
+                 /\ Forall2 (sem_var_instant (restr H k)) xs (xss k)))
+       \/
+       (exists xs ck f arg r ck_r ls x M' xss ys,
+           eq = EqApp xs ck f arg (Some (r, ck_r))
+           /\ Some x = hd_error xs
+           /\ msem_node G f (or_str rk (reset_of ys)) ls M' xss
+           /\ (forall k,
+                 sub_inst x (M k) (M' k)
+                 /\ sem_laexps_instant (bk k) (restr H k) ck arg (ls k)
+                 /\ Forall2 (sem_var_instant (restr H k)) xs (xss k)
+                 /\ sem_avar_instant (bk k) (restr H k) ck_r r (ys k)))
+       \/
+       (exists x ck c0 le ls xs,
+           eq = EqFby x ck c0 le
+           /\ mfby rk x (sem_const c0) ls M xs
+           /\ (forall k,
+                 sem_laexp_instant (bk k) (restr H k) ck le (ls k)
+                 /\ sem_var_instant (restr H k) x (xs k)))) ->
+      msem_equation G bk rk H M eq.
+  Proof.
+    induction eq; intros ** [Spec | [Spec | [Spec | Spec]]];
+      repeat destruct Spec as [? Spec]; try discriminate;
+        try match goal with
+          | H: EqDef _ _ _ = EqDef _ _ _ |- _ => inv H
+          | H: EqApp _ _ _ _ _ = EqApp _ _ _ _ _ |- _ => inv H
+          | H: EqFby _ _ _ _ = EqFby _ _ _ _ |- _ => inv H
+        end;
+        econstructor; unfold sem_var, sem_caexp, lift;
+          try (intro k; specialize (Spec k); intuition eauto); auto.
+  Qed.
+
+  Lemma instant_inv_msem_node:
+    forall G f rk xss M yss n H bk,
+      clock_of xss bk ->
+      find_node f G = Some n ->
+      (forall k, Forall2 (sem_var_instant (restr H k)) (map fst (n_in n)) (xss k)
+            /\ Forall2 (sem_var_instant (restr H k)) (map fst (n_out n)) (yss k)
+            /\ instant_same_clock (xss k)
+            /\ instant_same_clock (yss k)
+            /\ (absent_list (xss k) <-> absent_list (yss k))) ->
+      Forall (msem_equation G bk rk H M) n.(n_eqs) ->
+      msem_node G f rk xss M yss.
+  Proof.
+    intros ** Spec ?; econstructor; eauto.
+    - unfold sem_vars, lift; intro k; specialize (Spec k); intuition.
+    - unfold sem_vars, lift; intro k; specialize (Spec k); intuition.
+    - unfold same_clock; intro k; specialize (Spec k); intuition.
+    - unfold same_clock; intro k; specialize (Spec k); intuition.
+    - intro k; specialize (Spec k); intuition.
+  Qed.
+
+  Require Import Coq.Logic.ClassicalChoice.
+  Require Import Coq.Logic.ConstructiveEpsilon.
+  Require Import Coq.Logic.Epsilon.
+  Require Import Coq.Logic.IndefiniteDescription.
+
   Theorem sem_msem_node:
     forall G f xs ys,
       Welldef_global G ->
       sem_node G f xs ys ->
-      exists M, msem_node G sfalse f xs M ys.
+      exists M, msem_node G f falses xs M ys.
   Proof.
     induction G as [|node].
     inversion 2;
@@ -791,25 +829,80 @@ dataflow memory for which the non-standard semantics holds true.
       eapply Forall_sem_equation_global_tl in Heqs; eauto.
       assert (forall f xs ys,
                  sem_node G f xs ys ->
-                 exists M, msem_node G sfalse f xs M ys) as IHG'
+                 exists M, msem_node G f falses xs M ys) as IHG'
           by auto.
       assert (forall f r xs ys,
                  sem_reset G f r xs ys ->
-                 exists M, msem_node G r f xs M ys) as IHG''.
+                 exists M, msem_node G f r xs M ys) as IHG''.
       { clear - IHG'.
         intros ** Sem.
         inversion_clear Sem as [???? Sem'].
-        assert (forall n, exists Mn, msem_node G sfalse f (mask (all_absent (xs 0)) n r xs)
-                                     Mn (mask (all_absent (ys 0)) n r ys))
-               by (intro n; specialize (Sem' n); apply IHG' in Sem'; auto).
+        assert (forall k, exists M', msem_node G f falses (mask (all_absent (xs 0)) k r xs) M'
+                                    (mask (all_absent (ys 0)) k r ys)) as Msem'
+            by (intro; specialize (Sem' k); apply IHG' in Sem'; auto).
+        assert (exists F, forall k, msem_node G f falses (mask (all_absent (xs 0)) k r xs) (F k)
+                                    (mask (all_absent (ys 0)) k r ys))
+          as (F & Msem).
+        {
+          (** Infinite Description  *)
+          now apply functional_choice in Msem'.
 
-        (* eexists. *)
-        (* constructor. *)
+          (** Epsilon  *)
+          (* assert (inhabited memories) as I *)
+          (*     by (constructor; exact (fun n => @empty_memory val)). *)
+          (* exists (fun n => epsilon *)
+          (*            I (fun M => msem_node G f (mask (all_absent (xs 0)) n r xs) M *)
+          (*                               (mask (all_absent (ys 0)) n r ys))). *)
+          (* intro; now apply epsilon_spec.  *)
+
+          (** Constructive Epsilon  *)
+          (* pose proof (constructive_ground_epsilon memories) as F. *)
+
+          (** Classical Choice  *)
+          (* now apply choice in Msem'.   *)
+        }
+        clear Msem'.
+
+        exists (fun n => F (count r n) n).
+        pose proof (Msem 0) as Msem'.
+        inversion_clear Msem' as [???????? Hck Hf Hin Hout Hsx Hsy Habs Heqs];
+          clear Hck Hin Hout Hsx Hsy Habs Heqs.
+        assert (H': history) by admit.
+        eapply instant_inv_msem_node with (H := H'); eauto.
+        - eapply clock_of_equiv.
+        - intro k; specialize (Msem (count r k));
+            inversion_clear Msem as [???????? Hck Hf' Hin Hout Hsx Hsy Habs Heqs];
+            rewrite Hf in Hf'; inv Hf'.
+          unfold sem_vars, lift, same_clock in *;
+            specialize (Hin k); specialize (Hout k);
+              specialize (Hsx k); specialize (Hsy k); specialize (Habs k).
+          rewrite mask_transparent in Hin, Hout, Hsx, Hsy, Habs, Habs; auto.
+          intuition.
+          admit.
+          admit.
+        - apply Forall_forall.
+          intros eq Hin_eq.
+          apply instant_inv_msem_equation.
+          induction eq.
+          + left.
+            do 4 eexists; split; eauto.
+            intro k; specialize (Msem (count r k));
+              inversion_clear Msem as [???????? Hck Hf' Hin Hout Hsx Hsy Habs Heqs];
+              rewrite Hf in Hf'; inv Hf'.
+            rewrite Forall_forall in Heqs; apply Heqs in Hin_eq.
+            inv Hin_eq.
+            instantiate (1 := xs0).
+
+          SearchAbout Forall.
+          unfold restr.
+          eexact Hin.
+          SearchAbout mask count.
         admit.
       }
+
       inversion_clear Hwdef as [|??? neqs].
       simpl in neqs; unfold neqs in *.
-      assert (exists M', Forall (msem_equation G bk sfalse H M') n.(n_eqs))
+      assert (exists M', Forall (msem_equation G bk falses H M') n.(n_eqs))
         as (M & Hmsem) by now eapply sem_msem_eqs; eauto.
       exists M.
       econstructor; eauto.
@@ -827,8 +920,8 @@ dataflow memory for which the non-standard semantics holds true.
   with no return arguments. This is a bit of a hack, if you ask me. So
   don't ask. *)
   Lemma non_trivial_EqApp:
-    forall G bk H M eqs ,
-      Forall (msem_equation G bk H M) eqs ->
+    forall G bk rk H M eqs ,
+      Forall (msem_equation G bk rk H M) eqs ->
       forall ck f les y, ~ In (EqApp [] ck f les y) eqs.
   Proof.
   induction eqs; intros ** Hsem ? ? ? ? Hin.
